library/init/coe.lean
@@ -31,15 +31,7 @@ universes u v
 class has_lift (a : Sort u) (b : Sort v) :=
 (lift : a → b)
 
-/-- Auxiliary class that contains the transitive closure of has_lift. -/
-class has_lift_t (a : Sort u) (b : Sort v) :=
-(lift : a → b)
-
 class has_coe (a : Sort u) (b : Sort v) :=
-(coe : a → b)
-
-/-- Auxiliary class that contains the transitive closure of has_coe. -/
-class has_coe_t (a : Sort u) (b : Sort v) :=
 (coe : a → b)
 
 class has_coe_to_fun (a : Sort u) : Sort (max u (v+1)) :=
@@ -48,25 +40,10 @@ class has_coe_to_fun (a : Sort u) : Sort (max u (v+1)) :=
 class has_coe_to_sort (a : Sort u) : Type (max u (v+1)) :=
 (S : Sort v) (coe : a → S)
 
-def lift {a : Sort u} {b : Sort v} [has_lift a b] : a → b :=
-@has_lift.lift a b _
-
-def lift_t {a : Sort u} {b : Sort v} [has_lift_t a b] : a → b :=
-@has_lift_t.lift a b _
-
-def coe_b {a : Sort u} {b : Sort v} [has_coe a b] : a → b :=
-@has_coe.coe a b _
-
-def coe_t {a : Sort u} {b : Sort v} [has_coe_t a b] : a → b :=
-@has_coe_t.coe a b _
-
-def coe_fn_b {a : Sort u} [has_coe_to_fun.{u v} a] : Π x : a, has_coe_to_fun.F.{u v} x :=
-has_coe_to_fun.coe
-
 /- User level coercion operators -/
 
-@[reducible] def coe {a : Sort u} {b : Sort v} [has_lift_t a b] : a → b :=
-lift_t
+@[reducible] def coe {a : Sort u} {b : Sort v} [has_lift a b] : a → b :=
+has_lift.lift
 
 @[reducible] def coe_fn {a : Sort u} [has_coe_to_fun.{u v} a] : Π x : a, has_coe_to_fun.F.{u v} x :=
 has_coe_to_fun.coe
@@ -84,63 +61,13 @@ notation `↥`:max x:max := coe_sort x
 
 universes u₁ u₂ u₃
 
-/- Transitive closure for has_lift, has_coe, has_coe_to_fun -/
-
-instance lift_trans {a : Sort u₁} {b : Sort u₂} {c : Sort u₃} [has_lift_t b c] [has_lift a b] : has_lift_t a c :=
-⟨λ x, lift_t (lift x : b)⟩
-
-instance lift_base {a : Sort u} {b : Sort v} [has_lift a b] : has_lift_t a b :=
-⟨lift⟩
-
-instance coe_trans {a : Sort u₁} {b : Sort u₂} {c : Sort u₃} [has_coe_t b c] [has_coe a b] : has_coe_t a c :=
-⟨λ x, coe_t (coe_b x : b)⟩
-
-instance coe_base {a : Sort u} {b : Sort v} [has_coe a b] : has_coe_t a b :=
-⟨coe_b⟩
-
-/- We add this instance directly into has_coe_t to avoid non-termination.
-
-   Suppose coe_option had type (has_coe a (option a)).
-   Then, we can loop when searching a coercion from α to β (has_coe_t α β)
-   1- coe_trans at (has_coe_t α β)
-          (has_coe α ?b₁) and (has_coe_t ?b₁ c)
-   2- coe_option at (has_coe α ?b₁)
-          ?b₁ := option α
-   3- coe_trans at (has_coe_t (option α) β)
-          (has_coe (option α) ?b₂) and (has_coe_t ?b₂ β)
-   4- coe_option at (has_coe (option α) ?b₂)
-          ?b₂ := option (option α))
-   ...
--/
-instance coe_option {a : Type u} : has_coe_t a (option a) :=
+instance coe_option {a : Type u} : has_coe a (option a) :=
 ⟨λ x, some x⟩
-
-/- Auxiliary transitive closure for has_coe which does not contain
-   instances such as coe_option.
-
-   They would produce non-termination when combined with coe_fn_trans and coe_sort_trans.
--/
-class has_coe_t_aux (a : Sort u) (b : Sort v) :=
-(coe : a → b)
-
-instance coe_trans_aux {a : Sort u₁} {b : Sort u₂} {c : Sort u₃} [has_coe_t_aux b c] [has_coe a b] : has_coe_t_aux a c :=
-⟨λ x : a, @has_coe_t_aux.coe b c _ (coe_b x)⟩
-
-instance coe_base_aux {a : Sort u} {b : Sort v} [has_coe a b] : has_coe_t_aux a b :=
-⟨coe_b⟩
-
-instance coe_fn_trans {a : Sort u₁} {b : Sort u₂} [has_coe_to_fun.{u₂ u₃} b] [has_coe_t_aux a b] : has_coe_to_fun.{u₁ u₃} a :=
-{ F   := λ x, @has_coe_to_fun.F.{u₂ u₃} b _ (@has_coe_t_aux.coe a b _ x),
-  coe := λ x, coe_fn (@has_coe_t_aux.coe a b _ x) }
-
-instance coe_sort_trans {a : Sort u₁} {b : Sort u₂} [has_coe_to_sort.{u₂ u₃} b] [has_coe_t_aux a b] : has_coe_to_sort.{u₁ u₃} a :=
-{ S   := has_coe_to_sort.S.{u₂ u₃} b,
-  coe := λ x, coe_sort (@has_coe_t_aux.coe a b _ x) }
 
 /- Every coercion is also a lift -/
 
-instance coe_to_lift {a : Sort u} {b : Sort v} [has_coe_t a b] : has_lift_t a b :=
-⟨coe_t⟩
+instance coe_to_lift {a : Sort u} {b : Sort v} [has_coe a b] : has_lift a b :=
+⟨has_coe.coe⟩
 
 /- basic coercions -/
 
@@ -165,25 +92,23 @@ instance coe_subtype {a : Sort u} {p : a → Prop} : has_coe {x // p x} a :=
 
 universes ua ua₁ ua₂ ub ub₁ ub₂
 
-/- Remark: we can't use [has_lift_t a₂ a₁] since it will produce non-termination whenever a type class resolution
-   problem does not have a solution. -/
-instance lift_fn {a₁ : Sort ua₁} {a₂ : Sort ua₂} {b₁ : Sort ub₁} {b₂ : Sort ub₂} [has_lift a₂ a₁] [has_lift_t b₁ b₂] : has_lift (a₁ → b₁) (a₂ → b₂) :=
+instance lift_fn {a₁ : Sort ua₁} {a₂ : Sort ua₂} {b₁ : Sort ub₁} {b₂ : Sort ub₂} [has_lift a₂ a₁] [has_lift b₁ b₂] : has_lift (a₁ → b₁) (a₂ → b₂) :=
 ⟨λ f x, ↑(f ↑x)⟩
 
-instance lift_fn_range {a : Sort ua} {b₁ : Sort ub₁} {b₂ : Sort ub₂} [has_lift_t b₁ b₂] : has_lift (a → b₁) (a → b₂) :=
+instance lift_fn_range {a : Sort ua} {b₁ : Sort ub₁} {b₂ : Sort ub₂} [has_lift b₁ b₂] : has_lift (a → b₁) (a → b₂) :=
 ⟨λ f x, ↑(f x)⟩
 
 instance lift_fn_dom {a₁ : Sort ua₁} {a₂ : Sort ua₂} {b : Sort ub} [has_lift a₂ a₁] : has_lift (a₁ → b) (a₂ → b) :=
 ⟨λ f x, f ↑x⟩
 
-instance lift_pair {a₁ : Type ua₁} {a₂ : Type ub₂} {b₁ : Type ub₁} {b₂ : Type ub₂} [has_lift_t a₁ a₂] [has_lift_t b₁ b₂] : has_lift (a₁ × b₁) (a₂ × b₂) :=
-⟨λ p, prod.cases_on p (λ x y, (↑x, ↑y))⟩
+instance lift_pair {a₁ : Type ua₁} {a₂ : Type ub₂} {b₁ : Type ub₁} {b₂ : Type ub₂} [has_lift a₁ a₂] [has_lift b₁ b₂] : has_lift (a₁ × b₁) (a₂ × b₂) :=
+⟨λ p, p.map coe coe⟩
 
-instance lift_pair₁ {a₁ : Type ua₁} {a₂ : Type ua₂} {b : Type ub} [has_lift_t a₁ a₂] : has_lift (a₁ × b) (a₂ × b) :=
-⟨λ p, prod.cases_on p (λ x y, (↑x, y))⟩
+instance lift_pair₁ {a₁ : Type ua₁} {a₂ : Type ua₂} {b : Type ub} [has_lift a₁ a₂] : has_lift (a₁ × b) (a₂ × b) :=
+⟨λ p, p.map coe (λ x, x)⟩
 
-instance lift_pair₂ {a : Type ua} {b₁ : Type ub₁} {b₂ : Type ub₂} [has_lift_t b₁ b₂] : has_lift (a × b₁) (a × b₂) :=
-⟨λ p, prod.cases_on p (λ x y, (x, ↑y))⟩
+instance lift_pair₂ {a : Type ua} {b₁ : Type ub₁} {b₂ : Type ub₂} [has_lift b₁ b₂] : has_lift (a × b₁) (a × b₂) :=
+⟨λ p, p.map (λ x, x) coe⟩
 
-instance lift_list {a : Type u} {b : Type v} [has_lift_t a b] : has_lift (list a) (list b) :=
-⟨λ l, list.map (@coe a b _) l⟩
+instance lift_list {a : Type u} {b : Type v} [has_lift a b] : has_lift (list a) (list b) :=
+⟨λ l, l.map coe⟩
