library/init/category/lift.lean
@@ -21,27 +21,17 @@ universes u v w
 class has_monad_lift (m : Type u → Type v) (n : Type u → Type w) :=
 (monad_lift : ∀ {α}, m α → n α)
 
-/-- The reflexive-transitive closure of `has_monad_lift`.
-    `monad_lift` is used to transitively lift monadic computations such as `state_t.get` or `state_t.put s`.
-    Corresponds to [MonadLift](https://hackage.haskell.org/package/layers-0.1/docs/Control-Monad-Layer.html#t:MonadLift). -/
-class has_monad_lift_t (m : Type u → Type v) (n : Type u → Type w) :=
-(monad_lift : ∀ {α}, m α → n α)
-
-export has_monad_lift_t (monad_lift)
+export has_monad_lift (monad_lift)
 
 /-- A coercion that may reduce the need for explicit lifting.
     Because of [limitations of the current coercion resolution](https://github.com/leanprover/lean/issues/1402), this definition is not marked as a global instance and should be marked locally instead. -/
-@[reducible] def has_monad_lift_to_has_coe {m n} [has_monad_lift_t m n] {α} : has_coe (m α) (n α) :=
+@[reducible] def has_monad_lift_to_has_coe {m n} [has_monad_lift m n] {α} : has_coe (m α) (n α) :=
 ⟨monad_lift⟩
 
-instance has_monad_lift_t_trans (m n o) [has_monad_lift_t m n] [has_monad_lift n o] : has_monad_lift_t m o :=
-⟨λ α ma, has_monad_lift.monad_lift (monad_lift ma : n α)⟩
-
-instance has_monad_lift_t_refl (m) : has_monad_lift_t m m :=
+instance has_monad_lift_refl (m) : has_monad_lift m m :=
 ⟨λ α, id⟩
 
 @[simp] lemma monad_lift_refl {m : Type u → Type v} {α} : (monad_lift : m α → m α) = id := rfl
-
 
 /-- A functor in the category of monads. Can be used to lift monad-transforming functions.
     Based on pipes' [MFunctor](https://hackage.haskell.org/package/pipes-2.4.0/docs/Control-MFunctor.html),
@@ -50,23 +40,12 @@ instance has_monad_lift_t_refl (m) : has_monad_lift_t m m :=
 class monad_functor (m m' : Type u → Type v) (n n' : Type u → Type w) :=
 (monad_map {α : Type u} : (∀ {α}, m α → m' α) → n α → n' α)
 
-/-- The reflexive-transitive closure of `monad_functor`.
-    `monad_map` is used to transitively lift monad morphisms such as `state_t.zoom`.
-    A generalization of [MonadLiftFunctor](http://duairc.netsoc.ie/layers-docs/Control-Monad-Layer.html#t:MonadLiftFunctor), which can only lift endomorphisms (i.e. m = m', n = n'). -/
-class monad_functor_t (m m' : Type u → Type v) (n n' : Type u → Type w) :=
-(monad_map {α : Type u} : (∀ {α}, m α → m' α) → n α → n' α)
+export monad_functor (monad_map)
 
-export monad_functor_t (monad_map)
-
-instance monad_functor_t_trans (m m' n n' o o') [monad_functor_t m m' n n'] [monad_functor n n' o o'] :
-  monad_functor_t m m' o o' :=
-⟨λ α f, monad_functor.monad_map (λ α, (monad_map @f : n α → n' α))⟩
-
-instance monad_functor_t_refl (m m') : monad_functor_t m m' m m' :=
+instance monad_functor_refl (m m') : monad_functor m m' m m' :=
 ⟨λ α f, f⟩
 
 @[simp] lemma monad_map_refl {m m' : Type u → Type v} (f : ∀ {α}, m α → m' α) {α} : (monad_map @f : m α → m' α) = f := rfl
-
 
 /-- Run a monad stack to completion.
     `run` should be the composition of the transformers' individual `run` functions.
